src/klas/Klas.Rot.fst
@@ -9,6 +9,7 @@ open Kuiper.Tensor.Layout.Alg { l1_forward }
 open Kuiper.Complex32
 open Kuiper.Complex64
 open Kuiper.Complex.Class { complex, of_real }
+module CC = Kuiper.Complex.Class
 module Map = Kuiper.Kernel.Map
 
 inline_for_extraction noextract
@@ -60,3 +61,28 @@ fn csrot_gen (#c #r:Type0) {| scalar c |} {| floating r |} {| complex c r |}
 
 let csrot_cf32 = csrot_gen #cf32 #f32
 let csrot_cf64 = csrot_gen #cf64 #f64
+
+(* Crot/Zrot: real cosine, COMPLEX sine; needs conj + complex subtraction. *)
+inline_for_extraction noextract
+fn crot_gen (#c #r:Type0) {| scalar c |} {| floating r |} {| complex c r |}
+  (cc : r) (ss : c)
+  (lena : szp { lena <= max_blocks * max_threads })
+  (x : array1 c (l1_forward lena) { is_global x })
+  (y : array1 c (l1_forward lena) { is_global y })
+  (#vx : erased (lseq c lena))
+  (#vy : erased (lseq c lena))
+  preserves cpu
+  requires
+    on gpu_loc (x |-> vx) ** on gpu_loc (y |-> vy)
+  ensures
+    on gpu_loc (x |-> s_crot_x cc ss vx vy) ** on gpu_loc (y |-> s_crot_y cc ss vx vy)
+{
+  let tmp = alloc0 #c lena (l1_forward lena);
+  memcpy_device_to_device tmp x lena;
+  Map.map_gpu2 (fun (xi yi : c) -> add (mul (of_real cc) xi) (mul ss yi)) lena x y;
+  Map.map_gpu2 (fun (yi ti : c) -> CC.csub #c #r (mul (of_real cc) yi) (mul (CC.cconj #c #r ss) ti)) lena y tmp;
+  free tmp;
+}
+
+let crot_cf32 = crot_gen #cf32 #f32
+let crot_cf64 = crot_gen #cf64 #f64
